factored unification definitions and proofs out of monomorphic and polymorphic modules

Hindley-Milner.v
@@ -58,6 +58,252 @@ Module IS := WS.Make(IdDec).
 Module ISF := MSF.WFactsOn(IdDec)(IS).
 Module ISP := MSP.WPropertiesOn(IdDec)(IS).
 
+Module TypeSyntax.
+    Inductive type : Type :=
+        | TUnit
+        | TVar (X : id)
+        | TFun (t1 t2 : type).
+
+    Definition names : Type := IS.t.
+
+    Fixpoint fv (t : type) : names :=
+        match t with
+        | TUnit => IS.empty
+        | TVar X => IS.singleton X
+        | TFun t1 t2 => IS.union (fv t1) (fv t2)
+        end.
+
+    (* type variable in a type *)
+    Fixpoint TIn (X : id) (t : type) : Prop :=
+        match t with
+        | TUnit => False
+        | TVar Y => X = Y
+        | TFun t1 t2 => TIn X t1 \/ TIn X t2
+        end.
+End TypeSyntax.
+Export TypeSyntax.
+
+(* Signature for type substitution. *)
+Module Type Sigma.
+    (* Sigma: maps type variables 
+        to monomorphic types. *)
+    Parameter t : Type.
+    
+    Parameter empty : t.
+
+    Parameter bind : id -> type -> t -> t.
+
+    Parameter get : id -> t -> option type.
+
+    Axiom get_empty :
+        forall (X : id), get X empty = None.
+
+    Axiom bind_correct :
+        forall (X : id) (ty : type) (s : t),
+        get X (bind X ty s) = Some ty.
+
+    Axiom bind_complete :
+        forall {X Y : id}, Y <> X ->
+        forall (s : t) (ty : type),
+        get X (bind Y ty s) = get X s.
+
+    (* Sigma composition:
+        compose s1 s2 X = s2(s1(X)) *)
+    Parameter compose : t -> t -> t.
+
+    Axiom compose_empty :
+        forall (s : t),
+        compose empty s = s.
+
+    Fixpoint sub_type (s : t) (t : type) : type :=
+        match t with
+        | TUnit => TUnit
+        | TVar X => 
+            match get X s with
+            | None => TVar X
+            | Some t' => t'
+            end
+        | TFun t1 t2 => TFun (sub_type s t1) (sub_type s t2)
+        end.
+
+    Axiom compose_correct :
+        forall (s1 s2 : t) (ty : type),
+        sub_type (compose s1 s2) ty = (sub_type s2 (sub_type s1 ty)).
+
+    Axiom sub_type_bind_notin :
+        forall (X : id) (ty : type),
+        ~ TIn X ty ->
+        forall (T : type),
+        sub_type (bind X T empty) ty = ty.
+End Sigma.
+
+Module SigmaSubstitution(S : Sigma).
+    Lemma sub_type_empty :
+        forall (t : type),
+        S.sub_type S.empty t = t.
+    Proof.
+        intros t. induction t; 
+        try reflexivity; simpl.
+        - rewrite S.get_empty. reflexivity.
+        - rewrite IHt1. rewrite IHt2. reflexivity.
+    Qed.
+
+    Lemma sub_type_bind :
+        forall (X : id) (ty : type) (s : S.t),
+        ~ TIn X ty ->
+        S.sub_type (S.compose (S.bind X ty S.empty) s) (TVar X) =
+            S.sub_type (S.compose (S.bind X ty S.empty) s) ty.
+    Proof.
+        intros X ty s HIn.
+        rewrite S.compose_correct.
+        rewrite S.compose_correct. simpl. 
+        destruct (X =? X)%string eqn:eq; 
+        simpl in *.
+        - rewrite S.bind_correct. 
+            rewrite S.sub_type_bind_notin; auto.
+        - apply eqb_neq in eq. contradiction.
+    Qed.
+
+    Lemma sub_type_bind_inj :
+        forall (s : S.t) (X : id) (ty T : type),
+        S.sub_type s (S.sub_type (S.bind X ty S.empty) T) =
+        S.sub_type (S.compose (S.bind X ty S.empty) s) T.
+    Proof.
+        intros s X ty T. rewrite S.compose_correct.
+        reflexivity.
+    Qed.
+End SigmaSubstitution.
+
+Module ConstraintEquations.
+    Definition equation : Type := type * type.
+
+    Definition constraint : Type := list equation.
+
+    (* type variable in an equation *)
+    Fixpoint EQIn (X : id) (eq : equation) : Prop :=
+        let (t1,t2) := eq in TIn X t1 \/ TIn X t2.
+
+    (* type variable in a constraint *)
+    Definition CIn (X : id) (C : constraint) : Prop :=
+        Exists (EQIn X) C.
+End ConstraintEquations.
+Export ConstraintEquations.
+
+Module Unification(S : Sigma).
+    Module SS := SigmaSubstitution S.
+
+    Definition satisfy_equation (s : S.t) (eq : equation) : Prop :=
+        let (t1,t2) := eq in S.sub_type s t1 = S.sub_type s t2.
+
+    Definition satisfy_constraint (s : S.t) (C : constraint) : Prop :=
+    Forall (satisfy_equation s) C.
+
+    Definition sub_equation (s : S.t) (eq : equation) : equation :=
+            let (t1,t2) := eq in (S.sub_type s t1, S.sub_type s t2).
+
+    Definition sub_constraint (s : S.t) (C : constraint) : constraint :=
+        map (sub_equation s) C.
+
+    Inductive unify : constraint -> S.t -> Prop :=
+        | unify_nil : unify [] S.empty
+        | unify_eq : 
+            forall (t : type) (C : constraint) (s : S.t),
+            unify C s ->
+            unify ((t,t) :: C) s
+        | unify_left_var :
+            forall (X : id) (t : type) (C : constraint) (s : S.t),
+            ~ TIn X t ->
+            unify (sub_constraint (S.bind X t S.empty) C) s ->
+            unify ((TVar X, t) :: C) (S.compose (S.bind X t S.empty) s)
+        | unify_right_var :
+            forall (X : id) (t : type) (C : constraint) (s : S.t),
+            ~ TIn X t ->
+            unify (sub_constraint (S.bind X t S.empty) C) s ->
+            unify ((t, TVar X) :: C) (S.compose (S.bind X t S.empty) s)
+        | unify_fun : 
+            forall (a1 a2 b1 b2 : type) (C : constraint) (s : S.t),
+            unify ((a1,a2) :: (b1,b2) :: C) s ->
+            unify ((TFun a1 b1, TFun a2 b2) :: C) s.
+        
+    Definition more_general (s s' : S.t) : Prop :=
+        exists (s'' : S.t), s' = S.compose s s''.
+
+    Definition principal_unifier (C : constraint) (s : S.t) : Prop := 
+        satisfy_constraint s C /\ 
+        forall (s' : S.t), 
+        satisfy_constraint s' C ->  more_general s s'.
+
+    Lemma satisfy_equation_sym :
+        forall (s : S.t) (t1 t2 : type),
+        satisfy_equation s (t1,t2) ->
+        satisfy_equation s (t2,t1).
+    Proof.
+        intros s t1 t2 H. 
+        unfold satisfy_equation in *. auto.
+    Qed.
+
+    Lemma satisfy_constraint_compose :
+        forall (s : S.t) (X : id) (t : type) (C : constraint),
+        satisfy_constraint s (sub_constraint (S.bind X t S.empty) C) ->
+        satisfy_constraint (S.compose (S.bind X t S.empty) s) C.
+    Proof.
+        intros s X t C H.
+        unfold satisfy_constraint in *.
+        induction C; constructor; inv H; auto.
+        destruct a as [t1 t2].
+        unfold satisfy_equation in *.
+        simpl in H2. clear H3 IHC H.
+        rewrite <- SS.sub_type_bind_inj.
+        rewrite <- SS.sub_type_bind_inj.
+        assumption.
+    Qed.
+
+    Lemma satisfy_equation_compose :
+        forall (X : id) (t : type) (s : S.t),
+        ~ TIn X t ->
+        satisfy_equation (S.compose (S.bind X t S.empty) s) (TVar X, t).
+    Proof.
+        intros X t s HIn. unfold satisfy_equation.
+        apply SS.sub_type_bind; auto.
+    Qed.
+
+    Theorem unify_correct : 
+        forall (C : constraint) (s : S.t),
+        unify C s -> satisfy_constraint s C.
+    Proof.
+        intros C s HU. induction HU; constructor; auto.
+        - unfold satisfy_equation. reflexivity.
+        - apply satisfy_equation_compose. assumption.
+        - apply satisfy_constraint_compose. assumption.
+        - apply satisfy_equation_sym.
+            apply satisfy_equation_compose.
+            assumption.
+        - apply satisfy_constraint_compose. assumption.
+        - inv IHHU. simpl in *. rewrite H1. inv H2.
+            inv H3. rewrite H0. reflexivity.
+        - inv IHHU. inv H2. assumption.
+    Qed.
+    
+    Theorem unify_principal :
+        forall (C : constraint) (s : S.t),
+        unify C s -> principal_unifier C s.
+    Proof.
+        intros C s HU. unfold principal_unifier. split.
+        - apply unify_correct; auto.
+        - induction HU; try (intros s' HSC; unfold more_general).
+            + exists s'. rewrite S.compose_empty.
+                reflexivity.
+            + inv HSC. apply IHHU in H2. assumption.
+            + inv HSC. admit.
+            + admit.
+            + assert (H : satisfy_constraint 
+                s' ((a1, a2) :: (b1, b2) :: C)).
+                * inv HSC. inv H1.
+                    constructor; auto.
+                * apply IHHU in H. assumption.
+    Admitted.
+End Unification.
+
 Module Monomorphic.
     Section TypeMap.
         Context {T : Type}.
@@ -76,7 +322,7 @@ Module Monomorphic.
             intros. unfold bind. destruct ((x =? x)%string) eqn:eq.
             - reflexivity.
             - apply eqb_neq in eq. contradiction.
-        Qed. 
+        Qed.
 
         Lemma bind_complete :
             forall (x x' : id) (t t' : T),
@@ -110,33 +356,9 @@ Module Monomorphic.
                 - apply eqb_neq in eq. destruct ((y =? z)%string) eqn:eeq; reflexivity.
         Qed.
     End TypeMap.
+    Definition bind_correct_type := @bind_correct type.
 
     Module Syntax.
-        Module TypeSyntax.
-            Inductive type : Type :=
-                | TUnit
-                | TVar (X : id)
-                | TFun (t1 t2 : type).
-
-            Definition names : Type := IS.t.
-
-            Fixpoint fv (t : type) : names :=
-                match t with
-                | TUnit => IS.empty
-                | TVar X => IS.singleton X
-                | TFun t1 t2 => IS.union (fv t1) (fv t2)
-                end.
-    
-            (* type variable in a type *)
-            Fixpoint TIn (X : id) (t : type) : Prop :=
-                match t with
-                | TUnit => False
-                | TVar Y => X = Y
-                | TFun t1 t2 => TIn X t1 \/ TIn X t2
-                end.
-        End TypeSyntax.
-        Export TypeSyntax.
-
         Inductive expr : Type :=
             | EUnit
             | EVar (x : id)
@@ -174,63 +396,115 @@ Module Monomorphic.
                 check g (EApp e1 e2) t2.
     End TypeCheck.
 
-    Section TypeSubstitution.
-        Definition sigma : Type := @tmap type.
+    Module S <: Sigma.
+        Definition t : Type := @tmap type.
 
-        Fixpoint sub_type (s : sigma) (t : type) : type :=
+        Definition empty : t := tempty.
+        
+        Definition bind : id -> type -> t -> t := bind.
+    
+        Definition get (x :id) (s : S.t) : option type := s x.
+
+        Lemma bind_get_eta_eq :
+            forall (X Y : id) (s : t) (ty : type),
+            bind X ty s Y = get Y (bind X ty s).
+        Proof. intros X Y s ty. reflexivity. Qed.
+
+        Lemma get_empty :
+            forall (X : id), get X empty = None.
+        Proof. intros X. reflexivity. Qed.
+
+        Lemma bind_correct :
+            forall (x : id) (ty : type) (s : t),
+            get x (bind x ty s) = Some ty.
+        Proof. intros x ty s. apply bind_correct. Qed.
+
+        Lemma bind_complete :
+            forall {x y : id}, y <> x ->
+            forall (s : t) (ty : type),
+            get x (bind y ty s) = get x s.
+        Proof.
+            intros x y Hxy s ty. unfold get.
+            unfold bind. unfold Monomorphic.bind.
+            apply eqb_neq in Hxy. rewrite Hxy.
+            reflexivity.
+        Qed.
+
+        Fixpoint sub_type (s : t) (t : type) : type :=
             match t with
             | TUnit => TUnit
             | TVar X => 
-                match s X with
+                match get X s with
                 | None => TVar X
                 | Some t' => t'
                 end
             | TFun t1 t2 => TFun (sub_type s t1) (sub_type s t2)
             end.
 
-        Lemma sub_type_empty :
-            forall (t : type),
-            sub_type tempty t = t.
-        Proof.
-            intros t. induction t; try reflexivity.
-            simpl. rewrite IHt1. rewrite IHt2.
-            reflexivity.
-        Qed.
-
-        Definition sub_gamma (s : sigma) (g : gamma) : gamma :=
-            fun x =>
-                match g x with
-                | None => None
-                | Some t => Some (sub_type s t)
-                end.
-
-        (* s2(s1(X)) *)
-        Definition compose_sigma (s1 s2 : sigma) : sigma :=
+        Definition compose (s1 s2 : t) : t :=
             fun X => 
-                match s1 X with
-                | None => s2 X
+                match get X s1 with
+                | None => get X s2
                 | Some t => Some (sub_type s2 t)
                 end.
 
         Lemma compose_empty :
-            forall (s : sigma),
-            s = compose_sigma tempty s.
+            forall (s : t),
+            s = compose empty s.
         Proof.
             intros s. apply functional_extensionality.
             intros x. reflexivity.
         Qed.
 
-        Fixpoint sub_expr (s : sigma) (e : expr) : expr :=
+        Lemma compose_correct :
+            forall (s1 s2 : t) (ty : type),
+            sub_type (compose s1 s2) ty = (sub_type s2 (sub_type s1 ty)).
+        Proof.
+            intros s1 s2 ty. induction ty; 
+            auto; simpl.
+            - unfold compose; unfold get.
+                destruct (s1 X) eqn:eq; auto.
+            - rewrite IHty1. rewrite IHty2.
+                reflexivity.
+        Qed.
+
+        Lemma sub_type_bind_notin :
+            forall (X : id) (ty : type),
+            ~ TIn X ty ->
+            forall (T : type),
+            sub_type (bind X T empty) ty = ty.
+        Proof.
+            intros X ty. induction ty; 
+            intros HIn T; simpl in *; auto.
+            - rewrite bind_complete; auto.
+            - apply CP.not_or_and in HIn as [H1 H2].
+                apply IHty1 with (T := T) in H1.
+                apply IHty2 with (T := T) in H2.
+                rewrite H1. rewrite H2. reflexivity.
+        Qed.
+    End S.
+
+    Module SS := SigmaSubstitution S.
+
+    Section TypeSubstitution.
+        Definition sub_gamma (s : S.t) (g : gamma) : gamma :=
+            fun x =>
+                match g x with
+                | None => None
+                | Some t => Some (S.sub_type s t)
+                end.
+
+        Fixpoint sub_expr (s : S.t) (e : expr) : expr :=
             match e with
             | EUnit => EUnit
             | EVar x => EVar x
-            | EFun x t e => EFun x (sub_type s t) (sub_expr s e)
+            | EFun x t e => EFun x (S.sub_type s t) (sub_expr s e)
             | EApp e1 e2 => EApp (sub_expr s e1) (sub_expr s e2)
             end.
         
         Lemma bind_sub_gamma :
-            forall (s : sigma) (g : gamma) (x : id) (t : type),
-            sub_gamma s (bind x t g) = bind x (sub_type s t) (sub_gamma s g).
+            forall (s : S.t) (g : gamma) (x : id) (t : type),
+            sub_gamma s (bind x t g) = bind x (S.sub_type s t) (sub_gamma s g).
         Proof.
             intros s g x t. 
             apply functional_extensionality.
@@ -249,46 +523,28 @@ Module Monomorphic.
         Theorem substutution_preserves_typing :
             forall (g : gamma) (e : expr) (t : type),
             check g e t ->
-            forall (s : sigma),
-            check (sub_gamma s g) (sub_expr s e) (sub_type s t).
+            forall (s : S.t),
+            check (sub_gamma s g) (sub_expr s e) (S.sub_type s t).
         Proof.
             intros g e t H. induction H; intros s; try constructor.
             - unfold sub_gamma. rewrite H. reflexivity.
-            - fold sub_type. fold sub_expr.
+            - fold S.sub_type. fold sub_expr.
                 rewrite <- bind_sub_gamma.
                 apply IHcheck.
-            - apply check_app with (t1 := sub_type s t1);
+            - apply check_app with (t1 := S.sub_type s t1);
                 fold sub_expr; auto.
                 specialize IHcheck1 with (s := s).
                 simpl in IHcheck1. assumption.
         Qed.
 
-        Definition solution (g : gamma) (e : expr) (s : sigma) (t : type) : Prop :=
+        Definition solution (g : gamma) (e : expr) (s : S.t) (t : type) : Prop :=
         check (sub_gamma s g) (sub_expr s e) t.
     End TypeSubstitution.
 
+    Module U := Unification S.
+    Export U.
+
     Module ConstraintTyping.
-        Module ConstraintEquations.
-            Definition equation : Type := type * type.
-
-            Definition constraint : Type := list equation.
-
-            (* type variable in an equation *)
-            Fixpoint EQIn (X : id) (eq : equation) : Prop :=
-                let (t1,t2) := eq in TIn X t1 \/ TIn X t2.
-
-            (* type variable in a constraint *)
-            Definition CIn (X : id) (C : constraint) : Prop :=
-                Exists (EQIn X) C.
-        End ConstraintEquations.
-        Export ConstraintEquations.
-
-        Definition satisfy_equation (s : sigma) (eq : equation) : Prop :=
-                let (t1,t2) := eq in sub_type s t1 = sub_type s t2.
-            
-        Definition satisfy_constraint (s : sigma) (C : constraint) : Prop :=
-            Forall (satisfy_equation s) C.
-
         (* type variable not in gamma *)
         Definition GNIn (X : id) (g : gamma) : Prop :=
             forall (x : id) (t : type),
@@ -325,14 +581,14 @@ Module Monomorphic.
 
         Definition constraint_solution 
         {g : gamma} {e : expr} {t : type} {X : names} {C : constraint}
-        (H : constraint_type g e t X C) (s : sigma) (T : type) : Prop :=
-        satisfy_constraint s C /\ sub_type s t = T.
+        (H : constraint_type g e t X C) (s : S.t) (T : type) : Prop :=
+        satisfy_constraint s C /\ S.sub_type s t = T.
 
         Theorem Constraint_Typing_Sound : 
             forall (g : gamma) (e : expr) (t : type) 
                 (X : names) (C : constraint) 
                 (H : constraint_type g e t X C) 
-                (s : sigma) (T : type),
+                (s : S.t) (T : type),
             constraint_solution H s T -> solution g e s T.
         Proof.
             intros g e t X C H s T HCS.
@@ -343,11 +599,11 @@ Module Monomorphic.
             - apply substutution_preserves_typing.
                 constructor; auto.
             - constructor.
-                fold sub_type. fold sub_expr.
+                fold S.sub_type. fold sub_expr.
                 rewrite <- bind_sub_gamma. auto.
             - inv HSC.
                 apply Forall_app in H16 as [HC1 HC2].
-                apply check_app with (t1 := sub_type s t2); auto.
+                apply check_app with (t1 := S.sub_type s t2); auto.
                 fold sub_expr.
                 apply IHconstraint_type1 in HC1.
                 unfold satisfy_equation in H15.
@@ -356,17 +612,17 @@ Module Monomorphic.
         Qed.
 
         (* s/N *)
-        Definition sigma_diff (s : sigma) (N : names) : sigma := 
+        Definition sigma_diff (s : S.t) (N : names) : S.t := 
             fun X => if IS.mem X N then None else s X.
 
         Theorem Constraint_Typing_Complete : 
             forall (g : gamma) (e : expr) (t : type) 
             (X : names) (C : constraint) 
             (H : constraint_type g e t X C) 
-            (s : sigma) (T : type),
+            (s : S.t) (T : type),
             sigma_diff s X = s ->
             solution g e s T ->
-            exists (s' : sigma),
+            exists (s' : S.t),
             sigma_diff s' X = s /\ constraint_solution H s' T.
         Proof.
             intros g e t X C H.
@@ -376,154 +632,22 @@ Module Monomorphic.
     End ConstraintTyping.
     Export ConstraintTyping.
 
-    Section Unification.
-        Definition sub_equation (s : sigma) (eq : equation) : equation :=
-            let (t1,t2) := eq in (sub_type s t1, sub_type s t2).
-
-        Definition sub_constraint (s : sigma) (C : constraint) : constraint :=
-            map (sub_equation s) C.
-
-        Inductive unify : constraint -> sigma -> Prop :=
-            | unify_nil : unify [] tempty
-            | unify_eq : 
-                forall (t : type) (C : constraint) (s : sigma),
-                unify C s ->
-                unify ((t,t) :: C) s
-            | unify_left_var :
-                forall (X : id) (t : type) (C : constraint) (s : sigma),
-                ~ TIn X t ->
-                unify (sub_constraint (bind X t tempty) C) s ->
-                unify ((TVar X, t) :: C) (compose_sigma (bind X t tempty) s)
-            | unify_right_var :
-                forall (X : id) (t : type) (C : constraint) (s : sigma),
-                ~ TIn X t ->
-                unify (sub_constraint (bind X t tempty) C) s ->
-                unify ((t, TVar X) :: C) (compose_sigma (bind X t tempty) s)
-            | unify_fun : 
-                forall (a1 a2 b1 b2 : type) (C : constraint) (s : sigma),
-                unify ((a1,a2) :: (b1,b2) :: C) s ->
-                unify ((TFun a1 b1, TFun a2 b2) :: C) s.
-
-        Definition more_general (s s' : sigma) : Prop :=
-            exists (s'' : sigma), s' = compose_sigma s s''.
-
-        Definition principal_unifier (C : constraint) (s : sigma) : Prop := 
-            satisfy_constraint s C /\ 
-            forall (s' : sigma), 
-            satisfy_constraint s' C ->  more_general s s'.
-        
-        Lemma satisfy_equation_compose :
-            forall (X : id) (t : type) (s : sigma),
-            ~ TIn X t ->
-            satisfy_equation (compose_sigma (bind X t tempty) s) (TVar X, t).
-        Proof.
-            intros X t s H.
-            unfold satisfy_equation.
-            unfold compose_sigma. simpl.
-            rewrite bind_correct.
-            (* Intuitively true. *)
-            (* generalize dependent X. *)
-            (* generalize dependent s. *)
-            induction t; 
-            (* intros s X H;  *)
-            auto.
-            - assert (HXX : X <> X0).
-                + intros HF. apply H. subst.
-                    reflexivity.
-                + simpl. admit.
-            - simpl in H. 
-                apply CP.not_or_and in H as [H1 H2].
-                apply IHt1 in H1. apply IHt2 in H2.
-                simpl. rewrite H1. rewrite H2.
-                (* This case makes no sense. *)
-        Admitted.
-
-        Lemma satisfy_equation_sym :
-            forall (s : sigma) (t1 t2 : type),
-            satisfy_equation s (t1,t2) ->
-            satisfy_equation s (t2,t1).
-        Proof.
-            intros s t1 t2 H. 
-            unfold satisfy_equation in *. auto.
-        Qed.
-
-        Lemma satisfy_constraint_compose :
-            forall (s : sigma) (X : id) (t : type) (C : constraint),
-            satisfy_constraint s (sub_constraint (bind X t tempty) C) ->
-            satisfy_constraint (compose_sigma (bind X t tempty) s) C.
-        Proof.
-            intros s X t C H.
-            unfold satisfy_constraint in *.
-            induction C; constructor; inv H; auto.
-            destruct a as [t1 t2].
-            unfold satisfy_equation in *.
-            simpl in H2. clear H3 IHC H.
-            unfold compose_sigma.
-            destruct t1; destruct t2;
-            simpl in *; auto;
-            try destruct (sbind X t sempty X0); 
-            try destruct (sbind X t sempty X1);
-            auto; try discriminate.
-        Admitted.
-
-        Theorem unify_correct :
-            forall (C : constraint) (s : sigma),
-            unify C s -> principal_unifier C s.
-        Proof.
-            intros C s HU. unfold principal_unifier.
-            induction HU; split;
-            try (intros s' HSC; unfold more_general).
-            - constructor.
-            - exists s'. apply compose_empty.
-            - destruct IHHU as [HS _].
-                constructor; auto.
-                unfold satisfy_equation.
-                reflexivity.
-            - inv HSC. destruct IHHU as [_ IH].
-                apply IH in H2. assumption.
-            - destruct IHHU as [IH _].
-                constructor.
-                + apply satisfy_equation_compose. assumption.
-                + apply satisfy_constraint_compose. assumption.
-            - inv HSC. destruct IHHU as [_ IH]. admit.
-            - destruct IHHU as [IH _].
-                constructor.
-                + apply satisfy_equation_sym.
-                    apply satisfy_equation_compose.
-                    assumption.
-                + apply satisfy_constraint_compose. assumption.
-            - admit.
-            - destruct IHHU as [IH _]. inv IH.
-                inv H2. constructor; auto.
-                unfold satisfy_equation in *.
-                clear H2 H4. simpl.
-                rewrite H1. rewrite H3.
-                reflexivity.
-            - destruct IHHU as [_ IH].
-                assert (H : satisfy_constraint 
-                    s' ((a1, a2) :: (b1, b2) :: C)).
-                + inv HSC. inv H1.
-                    constructor; auto.
-                + apply IH in H. assumption.
-        Admitted.
-    End Unification.
-
     Section PrincipalTypes.
         Definition principal_solution
         {g : gamma} {e : expr} {t : type} {X : names} {C : constraint}
-        (H : constraint_type g e t X C) (s : sigma) (T : type) : Prop :=
+        (H : constraint_type g e t X C) (s : S.t) (T : type) : Prop :=
         constraint_solution H s T /\
-        forall (s' : sigma) (T' : type),
+        forall (s' : S.t) (T' : type),
         constraint_solution H s' T' -> more_general s s'.
 
         Corollary unify_principal_solution :
             forall {g : gamma} {e : expr} {t : type} {X : names} {C : constraint}
-                (H : constraint_type g e t X C) (s : sigma),
+                (H : constraint_type g e t X C) (s : S.t),
             unify C s ->
-            principal_solution H s (sub_type s t).
+            principal_solution H s (S.sub_type s t).
         Proof.
             intros g e t X C H s HU.
-            apply unify_correct in HU as HUC.
+            apply unify_principal in HU as HUC.
             unfold principal_unifier in HUC.
             unfold principal_solution.
             destruct HUC as [HSC HMG]. split.
@@ -535,9 +659,9 @@ Module Monomorphic.
 
         Lemma constraint_solution_unify :
             forall {g : gamma} {e : expr} {t : type} {X : names} {C : constraint}
-                (H : constraint_type g e t X C) (s' : sigma) (T' : type),
+                (H : constraint_type g e t X C) (s' : S.t) (T' : type),
             constraint_solution H s' T' ->
-            exists (s : sigma), unify C s.
+            exists (s : S.t), unify C s.
         Proof.
             intros g e t X C H s' T' HCS.
             unfold constraint_solution in HCS.
@@ -545,32 +669,32 @@ Module Monomorphic.
             dependent induction H; simpl in *;
             try (exists tempty; apply unify_nil).
             - apply IHconstraint_type
-                with (T' := sub_type s' t2) in HSC; auto.
+                with (T' := S.sub_type s' t2) in HSC; auto.
             - inv HSC. apply Forall_app in H16 as [HC1 HC2].
                 apply IHconstraint_type1 
-                    with (T' := sub_type s' t1) in HC1; auto.
+                    with (T' := S.sub_type s' t1) in HC1; auto.
                 apply IHconstraint_type2
-                    with (T' := sub_type s' t2) in HC2; auto.
+                    with (T' := S.sub_type s' t2) in HC2; auto.
                 destruct HC1 as [s1 HU1].
                 destruct HC2 as [s2 HU2].
                 destruct t1.
                 + inv H15.
-                + exists (compose_sigma (bind X0 (TFun t2 (TVar X)) tempty) (compose_sigma s1 s2)).
+                + exists (S.compose (S.bind X0 (TFun t2 (TVar X)) tempty) (S.compose s1 s2)).
                     constructor; admit.
-                + exists (compose_sigma s1 s2).
+                + exists (S.compose s1 s2).
                     constructor. admit.
         Admitted.
 
         Theorem principal_types :
             forall {g : gamma} {e : expr} {t : type} {X : names} {C : constraint}
                 (H : constraint_type g e t X C),
-            (exists (s' : sigma) (T' : type), constraint_solution H s' T') ->
-            exists (s : sigma) (T : type), principal_solution H s T.
+            (exists (s' : S.t) (T' : type), constraint_solution H s' T') ->
+            exists (s : S.t) (T : type), principal_solution H s T.
         Proof.
             intros g e t X C H [s' [T' HCS]].
             apply constraint_solution_unify in HCS.
             destruct HCS as [s HU].
-            exists s. exists (sub_type s t).
+            exists s. exists (S.sub_type s t).
             apply unify_principal_solution; auto.
         Qed.
 
@@ -587,27 +711,27 @@ Module Monomorphic.
                 interleave (bind x t1 g) e t2 ->
                 interleave g (EFun x t1 e) (TFun t1 t2)
             | il_app :
-                forall (e1 e2 : expr) (t1 t2 : type) (X : id) (s : sigma),
+                forall (e1 e2 : expr) (t1 t2 : type) (X : id) (s : S.t),
                 interleave g e1 t1 ->
                 interleave g e2 t2 ->
                 ~ TIn X t1 -> ~ TIn X t2 ->
                 ~ EIn X e1 -> ~ EIn X e2 -> GNIn X g ->
                 unify [(t1, TFun t2 (TVar X))] s ->
-                interleave g (EApp e1 e2) (sub_type s (TVar X)).
+                interleave g (EApp e1 e2) (S.sub_type s (TVar X)).
 
         Proposition interleave_sound :
             forall (g : gamma) (e : expr) (t : type),
             interleave g e t ->
             forall (N : names) (C : constraint)
                 (H : constraint_type g e t N C),
-            exists (s : sigma), unify C s /\ constraint_solution H s t.
+            exists (s : S.t), unify C s /\ constraint_solution H s t.
         Proof.
             intros g e t HIL. 
             induction HIL; intros N C HCT; inv HCT;
             unfold constraint_solution.
             - exists tempty. repeat split; constructor.
             - exists tempty. repeat split; 
-                try constructor. apply sub_type_empty.
+                try constructor. apply SS.sub_type_empty.
             - pose proof IHHIL N C H5 as IH.
                 destruct IH as [s [HU HCS]].
                 unfold constraint_solution in HCS.
@@ -638,23 +762,23 @@ Module Monomorphic.
         Definition e : expr := EApp (EVar f) (EVar a).
         
         Example ex2221 : 
-            solution g e (bind X (TFun (TVar Y) TUnit) tempty) TUnit.
+            solution g e (S.bind X (TFun (TVar Y) TUnit) tempty) TUnit.
         Proof. ex222 (TVar Y). Qed.
 
         Example ex2222 :
-            solution g e (bind X (TFun (TVar Y) (TVar Z)) (bind Z TUnit tempty)) (TVar Z).
+            solution g e (S.bind X (TFun (TVar Y) (TVar Z)) (S.bind Z TUnit tempty)) (TVar Z).
         Proof. ex222 (TVar Y). Qed.
 
         Example ex2223 :
-            solution g e (bind X (TFun TUnit TUnit) (bind Y TUnit tempty)) TUnit.
+            solution g e (S.bind X (TFun TUnit TUnit) (S.bind Y TUnit tempty)) TUnit.
         Proof. ex222 TUnit. Qed.
 
         Example ex224 :
-            solution g e (bind X (TFun (TVar Y) (TVar Z)) tempty) (TVar Z).
+            solution g e (S.bind X (TFun (TVar Y) (TVar Z)) tempty) (TVar Z).
         Proof. ex222 (TVar Y). Qed.
         
         Example ex2225 :
-            solution g e (bind X (TFun (TVar Y) (TFun TUnit TUnit)) tempty) (TFun TUnit TUnit).
+            solution g e (S.bind X (TFun (TVar Y) (TFun TUnit TUnit)) tempty) (TFun TUnit TUnit).
         Proof. ex222 (TVar Y). Qed.
 
         Definition term : expr := 
@@ -663,7 +787,7 @@ Module Monomorphic.
 
         Example ex2231 : 
             let s := (bind Y (TFun (TVar Z) TUnit) (bind X (TFun (TVar Z) (TFun TUnit TUnit)) tempty)) in
-            solution tempty term s (sub_type s (TFun (TVar X) (TFun (TVar Y) (TFun (TVar Z) TUnit)))).
+            solution tempty term s (S.sub_type s (TFun (TVar X) (TFun (TVar Y) (TFun (TVar Z) TUnit)))).
         Proof.
             unfold solution. simpl.
             repeat apply check_fun.
@@ -803,8 +927,6 @@ Module Monomorphic.
 End Monomorphic.
 
 Module Polymorphic.
-    Export Monomorphic.Syntax.TypeSyntax.
-
     Section Syntax.
         Inductive poly : Type :=
             | PType (t : type)
@@ -858,59 +980,149 @@ Module Polymorphic.
             | ELet (x : id) (e1 e2 : expr).
     End Syntax.
 
-    (* id map *)
-    Module IFM := FMW.Make(IdDec).
-    Module IFF := FMF.WFacts_fun(IdDec)(IFM).
+    Section TypeMap.
+        Context {T : Type}.
+
+        Definition tmap : Type := list (id * T).
+
+        Definition tempty : tmap := [].
+
+        Definition tbind (x : id) (t : T) (m : tmap) : tmap := (x, t) :: m.
+
+        Fixpoint tremove (x : id) (m : tmap) : tmap :=
+            match m with
+            | [] => []
+            | (y,t) :: m =>
+                if (y =? x)%string then (tremove x m) else (y,t) :: (tremove x m)
+            end.
+
+        Fixpoint tget (X : id) (m : tmap) : option T :=
+            match m with
+            | [] => None
+            | (Y,t)::m => if (Y =? X)%string then Some t else tget X m
+            end.
+    End TypeMap.
     
     (* typing context *)
-    Definition gamma : Type := IFM.t poly.
+    Definition gamma : Type := @tmap poly.
 
-    Section TypeSubstitution.
-        Definition sigma : Type := IFM.t type.
+    Module S <: Sigma.
+        Definition t : Type := @tmap type.
         
-        Fixpoint sub_type (s : sigma) (t : type) : type :=
+        Definition empty : t := tempty.
+
+        Definition bind : id -> type -> t -> t := tbind.
+        
+        Definition get : id -> t -> option type := tget.
+
+        Lemma get_empty : 
+            forall (X : id), get X empty = None.
+        Proof. intros X. reflexivity. Qed.
+
+        Lemma bind_correct :
+            forall (X : id) (ty : type) (s : t),
+            get X (bind X ty s) = Some ty.
+        Proof.
+            intros X ty s. cbn.
+            destruct (X =? X) eqn:eq; auto.
+            apply eqb_neq in eq. contradiction.
+        Qed.
+
+        Lemma bind_complete :
+            forall {X Y : id}, Y <> X ->
+            forall (s : t) (ty : type),
+            get X (bind Y ty s) = get X s.
+        Proof.
+            intros X Y HYX s ty. cbn.
+            apply eqb_neq in HYX. rewrite HYX.
+            reflexivity.
+        Qed.
+
+        Fixpoint sub_type (s : t) (t : type) : type :=
             match t with
             | TUnit => TUnit
-            | TVar X =>
-                match IFM.find X s with
+            | TVar X => 
+                match get X s with
                 | None => TVar X
                 | Some t' => t'
                 end
-            | TFun t1 t2 =>
-                TFun (sub_type s t1) (sub_type s t2)
+            | TFun t1 t2 => TFun (sub_type s t1) (sub_type s t2)
             end.
 
-        Fixpoint sub_expr (s : sigma) (e : expr) : expr :=
+        Lemma sub_type_empty :
+            forall (t : type),
+            sub_type empty t = t.
+        Proof.
+            intros t. induction t; try reflexivity. simpl. 
+            rewrite IHt1. rewrite IHt2. reflexivity.
+        Qed.
+
+        Fixpoint compose (s1 s2 : S.t) : S.t :=
+            match s1 with
+            | [] => s2
+            | (X, T) :: s1 => (X, sub_type s2 T) :: compose s1 s2
+            end.
+
+        Lemma compose_empty :
+            forall (s : t),
+            compose empty s = s.
+        Proof. intros s. reflexivity. Qed.
+
+        Lemma compose_correct :
+            forall (s1 s2 : t) (ty : type),
+            sub_type (compose s1 s2) ty = (sub_type s2 (sub_type s1 ty)).
+        Proof.
+            intros s1 s2 ty. induction ty; 
+            auto; simpl in *.
+            - induction s1; simpl; auto.
+                destruct a as [Y T]. simpl.
+                destruct (Y =? X) eqn:eq; auto.
+            - rewrite IHty1. rewrite IHty2.
+                reflexivity.
+        Qed.
+
+        Lemma sub_type_bind_notin :
+            forall (X : id) (ty : type),
+            ~ TIn X ty ->
+            forall (T : type),
+            sub_type (bind X T empty) ty = ty.
+        Proof.
+            intros X ty Hin T. induction ty; 
+            simpl in *; auto.
+            - apply eqb_neq in Hin. rewrite Hin.
+                reflexivity.
+            - apply CP.not_or_and in Hin as [H1 H2].
+                apply IHty1 in H1. apply IHty2 in H2.
+                rewrite H1. rewrite H2. reflexivity.
+        Qed.
+    End S.
+    
+    Section TypeSubstitution.
+        Fixpoint sub_expr (s : S.t) (e : expr) : expr :=
             match e with
             | EUnit => EUnit
             | EVar x => EVar x
-            | EFun x t e => EFun x (sub_type s t) (sub_expr s e)
+            | EFun x t e => EFun x (S.sub_type s t) (sub_expr s e)
             | EApp e1 e2 => EApp (sub_expr s e1) (sub_expr s e2)
             | ELet x e1 e2 => ELet x (sub_expr s e1) (sub_expr s e2)
             end.
 
-        Fixpoint sub_poly (s : sigma) (p : poly) : poly :=
+        Fixpoint sub_poly (s : S.t) (p : poly) : poly :=
             match p with
-            | PType t => PType (sub_type s t)
+            | PType t => PType (S.sub_type s t)
             | PForall X p =>
-                PForall X (sub_poly (IFM.remove X s) p)
+                PForall X (sub_poly (tremove X s) p)
             end.
 
-        Definition sub_gamma (s : sigma) : gamma -> gamma := IFM.map (sub_poly s).
-
-        (* s2(s1(t)) = t' *)
-        Definition compose_sigma (s1 s2 : sigma) : sigma :=
-            let s1' := IFM.map (sub_type s2) s1 in
-            IFM.fold
-                (fun X t acc => 
-                    if IFM.mem X s1' 
-                        then acc
-                        else IFM.add X t acc) s2 s1'.
+        Definition sub_gamma (s : S.t) : gamma -> gamma := 
+            map (fun (e : id * poly) =>
+                let (x,p) := e in (x, sub_poly s p)).
     End TypeSubstitution.
 
-    Section ConstraintTyping.
-        Import Monomorphic.ConstraintTyping.ConstraintEquations.
+    Module U := Unification S.
+    Export U.
 
+    Section ConstraintTyping.
         (* type name in a poly-type, accounting for bound type names *)
         Fixpoint PIn (X : id) (p : poly) : Prop :=
             match p with
@@ -918,16 +1130,15 @@ Module Polymorphic.
             | PForall Y p => X <> Y /\ PIn X p
             end.
 
-        Definition satisfy_equation (s : sigma) (eq : equation) : Prop :=
-                let (t1,t2) := eq in sub_type s t1 = sub_type s t2.
-            
-        Definition satisfy_constraint (s : sigma) (C : constraint) : Prop :=
-            Forall (satisfy_equation s) C.
+        (* type variable in gamma *)
+        Definition GIn (X : id) (g : gamma) : Prop :=
+            exists (x : id) (p : poly), 
+            tget x g = Some p /\ PIn X p.
 
         (* type variable not in gamma *)
         Definition GNIn (X : id) (g : gamma) : Prop :=
             forall (x : id) (p : poly), 
-            IFM.MapsTo x p g -> ~ PIn X p.
+            tget x g = Some p -> ~ PIn X p.
 
         (* type variable in an expression *)
         Fixpoint EIn (X : id) (e : expr) : Prop :=
@@ -939,18 +1150,41 @@ Module Polymorphic.
 
         (* complete substitution of a poly-type to get 
             a type with fresh type variables *)
-        Inductive sub_poly_type (g : gamma) (s : sigma) 
+        Inductive sub_poly_type (g : gamma) (s : S.t) 
         : poly -> type -> names -> constraint -> Prop :=
             | spt_type : 
                 forall (t t' : type), 
-                sub_type s t = t' ->
+                S.sub_type s t = t' ->
                 sub_poly_type g s (PType t) t' IS.empty []
             | spt_forall :
                 forall (X Y : id) (p : poly) 
                     (N : names) (C : constraint) (t : type),
                 GNIn Y g -> ~ PIn Y p -> ~ IS.In Y N ->
-                sub_poly_type g (IFM.add X (TVar Y) s) p t N C ->
+                sub_poly_type g (S.bind X (TVar Y) s) p t N C ->
                 sub_poly_type g s (PForall X p) t (IS.add Y N) ((TVar X, TVar Y) :: C).
+
+        Definition make_fun_poly (p1 p2 : poly) : poly :=
+            let (N1,t1') := to_scheme p1 in
+            let (N2,t2') := to_scheme p2 in
+            to_poly (N1 ++ N2, TFun t1' t2').
+
+        (* generalizes unbound type variables *)
+        Inductive generalize_names (g : gamma) : type -> poly -> Prop :=
+            | gun_unit : generalize_names g TUnit (PType TUnit)
+            | gun_var_bound :
+                forall (X : id),
+                GIn X g ->
+                generalize_names g (TVar X) (PType (TVar X))
+            | gun_var_free :
+                forall (X : id),
+                ~ GIn X g ->
+                generalize_names g (TVar X) (PForall X (PType (TVar X)))
+            | gun_fun :
+                forall (t1 t2 : type) (p1 p2 p : poly),
+                p = make_fun_poly p1 p2 ->
+                generalize_names g t1 p1 ->
+                generalize_names g t2 p2 ->
+                generalize_names g (TFun t1 t2) p.
 
         Inductive constraint_type (g : gamma) 
         : expr -> type -> names -> constraint -> Prop :=
@@ -959,13 +1193,13 @@ Module Polymorphic.
             | ct_var :
                 forall (x : id) (p : poly) (t : type) 
                     (N : names) (C : constraint),
-                IFM.MapsTo x p g ->
-                sub_poly_type g (@IFM.empty type) p t N C ->
+                tget x g = Some p ->
+                sub_poly_type g S.empty p t N C ->
                 constraint_type g (EVar x) t N C
             | ct_fun :
                 forall (x : id) (t1 t2 : type) 
                     (e : expr) (N : names) (C : constraint),
-                constraint_type (IFM.add x (PType t1) g) e t2 N C ->
+                constraint_type (tbind x (PType t1) g) e t2 N C ->
                 constraint_type g (EFun x t1 e) (TFun t1 t2) N C
             | ct_app :
                 forall (e1 e2 : expr) (t1 t2 : type) (X : id)
@@ -978,10 +1212,20 @@ Module Polymorphic.
                 ~ IS.In X N1 -> ~ IS.In X N2 ->
                 ~ TIn X t1 -> ~ TIn X t2 ->
                 ~ EIn X e1 -> ~ EIn X e2 ->
-                ~ CIn X C1 -> ~ CIn X C2 -> GNIn X g ->
+                ~ CIn X C1 -> ~ CIn X C2 -> ~ GIn X g ->
                 constraint_type g (EApp e1 e2) (TVar X)
                     (IS.add X (IS.union N1 N2))
-                    ((t1, TFun t2 (TVar X)) :: C1 ++ C2).
-            (* TODO: ct_let *)
+                    ((t1, TFun t2 (TVar X)) :: C1 ++ C2)
+            | ct_let :
+                forall (x : id) (e1 e2 : expr) (t1 t2 : type)
+                    (p1 : poly) (N1 N2 : names) (C1 C2 : constraint),
+                    constraint_type g e1 t1 N1 C1 ->
+                    generalize_names g t1 p1 ->
+                    constraint_type (tbind x p1 g) e2 t2 N2 C2 ->
+                    IS.Empty (IS.inter N1 N2) ->
+                    IS.Empty (IS.inter N1 (fv t2)) ->
+                    IS.Empty (IS.inter N2 (fv t1)) ->
+                    constraint_type g (ELet x e1 e2) t2
+                        (IS.union N1 N2) (C1 ++ C2).
     End ConstraintTyping.
 End Polymorphic.
